high-level recursor for LC

case_studies/Untyped_Lambda_Calculus/LC.thy
@@ -19,6 +19,194 @@ for
   subst: tvsubst
 print_theorems
 
+locale HL_REC_term =
+  fixes Pmap :: "('a :: var \<Rightarrow> 'a) \<Rightarrow> 'p \<Rightarrow> 'p"
+    and PFVars :: "'p \<Rightarrow> 'a set"
+    and validP :: "'p \<Rightarrow> bool"
+    and avoiding_set :: "'a set"
+    and Umap :: "('a \<Rightarrow> 'a) \<Rightarrow> 'a LC.term \<Rightarrow> 'u \<Rightarrow> 'u"
+    and UFVars :: "'a LC.term \<Rightarrow> 'u \<Rightarrow> 'a set"
+    and UVar :: "'a \<Rightarrow> 'p \<Rightarrow> 'u"
+    and UApp :: "'a LC.term \<Rightarrow> ('p \<Rightarrow> 'u) \<Rightarrow> 'a LC.term \<Rightarrow> ('p \<Rightarrow> 'u) \<Rightarrow> 'p \<Rightarrow> 'u"
+    and ULam :: "'a \<Rightarrow> 'a LC.term \<Rightarrow> ('p \<Rightarrow> 'u) \<Rightarrow> 'p \<Rightarrow> 'u"
+    and validU :: "'u \<Rightarrow> bool"
+  assumes
+    Pmap_comp: "\<And>d f g. validP d \<Longrightarrow>
+       bij f \<Longrightarrow>
+       |supp f| <o |UNIV :: 'a set| \<Longrightarrow>
+       bij g \<Longrightarrow>
+       |supp g| <o |UNIV :: 'a set| \<Longrightarrow>
+       Pmap (f \<circ> g) d = (Pmap f \<circ> Pmap g) d" and
+    Pmap_cong_id: "\<And>d f. validP d \<Longrightarrow>
+           bij f \<Longrightarrow>
+           |supp f| <o |UNIV :: 'a set| \<Longrightarrow>
+           (\<And>a. a \<in> PFVars d \<Longrightarrow> f a = a) \<Longrightarrow>
+           Pmap f d = d" and
+    PFVars_Pmap: "\<And>d f. validP d \<Longrightarrow>
+           bij f \<Longrightarrow>
+           |supp f| <o |UNIV :: 'a set| \<Longrightarrow>
+           PFVars (Pmap f d) = f ` PFVars d" and
+    card_of_PFVars: "validP p \<Longrightarrow> |PFVars p| <o |UNIV :: 'a set|" and
+    validP_Pmap: "validP p \<Longrightarrow>
+           bij f \<Longrightarrow>
+           |supp f| <o |UNIV :: 'a set| \<Longrightarrow>
+           validP (Pmap f p)" and
+    card_of_avoiding_set: "|avoiding_set| <o |UNIV :: 'a set|" and
+    Umap_comp: "\<And>d f g t.
+       validU d \<Longrightarrow>
+       bij f \<Longrightarrow>
+       |supp f| <o |UNIV :: 'a set| \<Longrightarrow>
+       bij g \<Longrightarrow>
+       |supp g| <o |UNIV :: 'a set| \<Longrightarrow>
+       Umap (f \<circ> g) t d =
+       (Umap f t \<circ> Umap g t) d" and
+    Umap_cong_id: "\<And>d t f.
+       validU d \<Longrightarrow>
+       bij f \<Longrightarrow>
+       |supp f| <o |UNIV :: 'a set| \<Longrightarrow>
+       (\<And>a. a \<in> UFVars t d \<Longrightarrow> f a = a) \<Longrightarrow>
+       Umap f t d = d" and
+    validU_Umap: "\<And>f t u.
+       validU u \<Longrightarrow>
+       bij f \<Longrightarrow>
+       |supp f| <o |UNIV :: 'a set| \<Longrightarrow>
+       validU (Umap f t u)" and
+    Umap_UVar: "\<And>p x f. validP p \<Longrightarrow>
+    bij f \<Longrightarrow>
+    |supp f| <o |UNIV :: 'a set| \<Longrightarrow>
+    imsupp f \<inter> avoiding_set = {} \<Longrightarrow>
+    Umap f (Var x) (UVar x p) = UVar (f x) (Pmap f p)" and
+    Umap_ULam: "\<And>p x t pu f. validP p \<Longrightarrow>
+    bij f \<Longrightarrow>
+    |supp f| <o |UNIV :: 'a set| \<Longrightarrow>
+    imsupp f \<inter> avoiding_set = {} \<Longrightarrow>
+    pred_fun validP validU pu \<Longrightarrow>
+    Umap f (Lam x t) (ULam x t pu p) = ULam (f x) (permute_term f t)
+      (\<lambda>p. if validP p then Umap f t (pu (Pmap (inv f) p)) else undefined) (Pmap f p)" and
+    Umap_UApp: "\<And>p t1 pu1 t2 pu2 f. validP p \<Longrightarrow>
+    bij f \<Longrightarrow>
+    |supp f| <o |UNIV :: 'a set| \<Longrightarrow>
+    imsupp f \<inter> avoiding_set = {} \<Longrightarrow>
+    pred_fun validP validU pu1 \<Longrightarrow>
+    pred_fun validP validU pu2 \<Longrightarrow>
+    Umap f (App t1 t2) (UApp t1 pu1 t2 pu2 p) = UApp
+      (permute_term f t1)
+      (\<lambda>p. if validP p then Umap f t1 (pu1 (Pmap (inv f) p)) else undefined)
+      (permute_term f t2)
+      (\<lambda>p. if validP p then Umap f t2 (pu2 (Pmap (inv f) p)) else undefined) (Pmap f p)"
+   and
+   UFVars_UVar: "\<And>p x. validP p \<Longrightarrow>
+   UFVars (Var x) (UVar x p) \<subseteq> FFVars (Var x) \<union> PFVars p \<union> avoiding_set"
+   and
+   UFVars_ULam: "\<And>p x t pu. validP p \<Longrightarrow>
+   pred_fun validP validU pu \<Longrightarrow>
+   {x} \<inter> (PFVars p \<union> avoiding_set) = {} \<Longrightarrow>
+   (\<And>p. validP p \<Longrightarrow> UFVars t (pu p) \<subseteq> FFVars t \<union> PFVars p \<union> avoiding_set) \<Longrightarrow>
+   UFVars (Lam x t) (ULam x t pu p) \<subseteq> FFVars (Lam x t) \<union> PFVars p \<union> avoiding_set"
+   and
+   UFVars_UApp: "\<And>p t1 pu1 t2 pu2. validP p \<Longrightarrow>
+   pred_fun validP validU pu1 \<Longrightarrow>
+   pred_fun validP validU pu2 \<Longrightarrow>
+   (\<And>p. validP p \<Longrightarrow> UFVars t1 (pu1 p) \<subseteq> FFVars t1 \<union> PFVars p \<union> avoiding_set) \<Longrightarrow>
+   (\<And>p. validP p \<Longrightarrow> UFVars t2 (pu2 p) \<subseteq> FFVars t2 \<union> PFVars p \<union> avoiding_set) \<Longrightarrow>
+   UFVars (App t1 t2) (UApp t1 pu1 t2 pu2 p) \<subseteq> FFVars (App t1 t2) \<union> PFVars p \<union> avoiding_set"
+  and
+    validU_UVar: "\<And>p x. validP p \<Longrightarrow> validU (UVar x p)" and
+    validU_ULam: "\<And>p x t pu. validP p \<Longrightarrow> pred_fun validP validU pu \<Longrightarrow> validU (ULam x t pu p)" and
+    validU_UApp: "\<And>p t1 pu1 t2 pu2. validP p \<Longrightarrow> pred_fun validP validU pu1 \<Longrightarrow> pred_fun validP validU pu2 \<Longrightarrow> validU (UApp t1 pu1 t2 pu2 p)"
+  begin
+
+definition "Uctor x = (case Rep_term_pre x of
+    Inl a \<Rightarrow> UVar a
+  | Inr (Inl ((t, trec), (u, urec))) \<Rightarrow> UApp t trec u urec
+  | Inr (Inr (x, (t, trec))) \<Rightarrow> ULam x t trec)"
+ 
+interpretation HL_to_LL: REC_term Pmap PFVars validP avoiding_set Umap UFVars Uctor validU
+  apply standard
+  apply (rule Pmap_comp; assumption)
+  apply (rule Pmap_cong_id; assumption)
+  apply (rule PFVars_Pmap; assumption)
+  apply (rule card_of_PFVars; assumption)
+  apply (rule validP_Pmap; assumption)
+  apply (rule card_of_avoiding_set; assumption)
+  apply (rule Umap_comp; assumption)
+      apply (rule Umap_cong_id; assumption)
+  subgoal for f y p
+    unfolding Uctor_def map_term_pre_def term_pre.pred_set set3_term_pre_def set4_term_pre_def
+    apply (auto simp: Var_def[symmetric] Lam_def[symmetric] App_def[symmetric]
+       Abs_term_pre_inverse
+       split: sum.splits intro!: Umap_UVar Umap_ULam Umap_UApp)
+    done
+  subgoal for y p
+    unfolding Uctor_def map_term_pre_def term_pre.pred_set set1_term_pre_def set2_term_pre_def set3_term_pre_def set4_term_pre_def
+    apply (auto simp: Var_def[symmetric] Lam_def[symmetric] App_def[symmetric]
+       Abs_term_pre_inverse
+       split: sum.splits 
+       del: subsetI simp del: term.set
+       intro!: UFVars_UVar UFVars_ULam UFVars_UApp)
+    done
+   apply (rule validU_Umap; assumption)
+  subgoal for y p
+    unfolding Uctor_def map_term_pre_def term_pre.pred_set set3_term_pre_def set4_term_pre_def
+        apply (auto simp: Var_def[symmetric] Lam_def[symmetric] App_def[symmetric]
+       Abs_term_pre_inverse
+       split: sum.splits intro!: validU_UVar validU_ULam validU_UApp)
+    done
+  done
+
+definition HL_REC_term where "HL_REC_term = HL_to_LL.REC_term"
+
+lemma HL_REC_term_Var: "validP p \<Longrightarrow> HL_REC_term (Var x) p = UVar x p"
+  unfolding Var_def HL_REC_term_def
+  apply (subst HL_to_LL.REC_ctor)
+  apply (auto simp: Uctor_def map_term_pre_def set2_term_pre_def Abs_term_pre_inverse noclash_term_def)
+  done
+
+lemma HL_REC_term_Lam: "validP p \<Longrightarrow> {x} \<inter> (PFVars p \<union> avoiding_set) = {} \<Longrightarrow>
+  HL_REC_term (Lam x t) p = ULam x t (\<lambda>p. if validP p then HL_REC_term t p else undefined) p"
+  unfolding Lam_def HL_REC_term_def
+  apply (subst HL_to_LL.REC_ctor)
+  apply (auto simp: Uctor_def map_term_pre_def set1_term_pre_def set2_term_pre_def set3_term_pre_def set4_term_pre_def Abs_term_pre_inverse noclash_term_def)
+  done
+
+lemma HL_REC_term_App: "validP p \<Longrightarrow>
+  HL_REC_term (App t1 t2) p = UApp t1 (\<lambda>p. if validP p then HL_REC_term t1 p else undefined) t2 (\<lambda>p. if validP p then HL_REC_term t2 p else undefined) p"
+  unfolding App_def HL_REC_term_def
+  apply (subst HL_to_LL.REC_ctor)
+  apply (auto simp: Uctor_def map_term_pre_def set1_term_pre_def set2_term_pre_def set3_term_pre_def set4_term_pre_def Abs_term_pre_inverse noclash_term_def)
+  done
+
+lemmas HL_REC_term_swap = HL_to_LL.REC_swap[folded HL_REC_term_def]
+lemmas HL_REC_term_UFVars = HL_to_LL.REC_UFVars[folded HL_REC_term_def]
+
+end
+
+context fixes x :: "'a :: var" begin
+interpretation HL_REC_term
+  where
+  Pmap = "\<lambda>f (u :: unit). u" and
+  PFVars = "\<lambda>(u :: unit). {}" and
+  validP = "\<lambda>(u :: unit). True" and
+  avoiding_set = "{x}" and
+  Umap = "\<lambda>f t (n :: nat). n" and
+  UFVars = "\<lambda>t (n :: nat). {}" and
+  validU = "\<lambda>(n :: nat). True" and
+  UVar = "\<lambda>y u. if x = y then (1 :: nat) else 0" and
+  UApp = "\<lambda>t1 pu1 t2 pu2 u. pu1 u + pu2 u" and
+  ULam = "\<lambda>y t pu u. pu u"
+  apply standard
+  apply (auto dest: notin_imsupp simp: in_imsupp)
+  done
+
+definition "count t = HL_REC_term t ()"
+lemmas count_simps[where p = "()", folded count_def, simplified] =
+  HL_REC_term_Var HL_REC_term_Lam HL_REC_term_App
+lemmas count_swap = HL_REC_term_swap[where p="()", folded count_def, simplified]
+
+end
+
+thm count_simps count_swap
+
 (****************************)
 (* DATATYPE-SPECIFIC CUSTOMIZATION  *)
 
